theories/caesium/lang.v
@@ -74,7 +74,8 @@ hardware threads). *)
 Inductive stmt :=
 | Goto (b : label)
 | Return (e : expr)
-| IfS (ot : op_type) (e : expr) (s1 s2 : stmt)
+(* join : label of the join point, only for informational purposes *)
+| IfS (ot : op_type) (join : option label) (e : expr) (s1 s2 : stmt)
 (* m: map from values of e to indices into bs, def: default *)
 | Switch (it : int_type) (e : expr) (m : gmap Z nat) (bs : list stmt) (def : stmt)
 | Assign (o : order) (ot : op_type) (e1 e2 : expr) (s : stmt)
@@ -134,7 +135,7 @@ with rtexpr :=
 with rtstmt :=
 | RTGoto (b : label)
 | RTReturn (e : runtime_expr)
-| RTIfS (ot : op_type) (e : runtime_expr) (s1 s2 : stmt)
+| RTIfS (ot : op_type) (join : option label) (e : runtime_expr) (s1 s2 : stmt)
 | RTSwitch (it : int_type) (e : runtime_expr) (m : gmap Z nat) (bs : list stmt) (def : stmt)
 | RTAssign (o : order) (ot : op_type) (e1 e2 : runtime_expr) (s : stmt)
 | RTFree (ly : layout) (e : runtime_expr) (s : stmt)
@@ -166,7 +167,7 @@ Definition to_rtstmt (rf : runtime_function) (s : stmt) : runtime_expr :=
   Stmt rf $ match s with
   | Goto b => RTGoto b
   | Return e => RTReturn (to_rtexpr e)
-  | IfS ot e s1 s2 => RTIfS ot (to_rtexpr e) s1 s2
+  | IfS ot join e s1 s2 => RTIfS ot join (to_rtexpr e) s1 s2
   | Switch it e m bs def => RTSwitch it (to_rtexpr e) m bs def
   | Assign o ot e1 e2 s => RTAssign o ot (to_rtexpr e1) (to_rtexpr e2) s
   | Free ly e s => RTFree ly (to_rtexpr e) s
@@ -219,7 +220,7 @@ Fixpoint subst_stmt (xs : list (var_name * val)) (s : stmt) : stmt :=
   match s with
   | Goto b => Goto b
   | Return e => Return (subst_l xs e)
-  | IfS ot e s1 s2 => IfS ot (subst_l xs e) (subst_stmt xs s1) (subst_stmt xs s2)
+  | IfS ot join e s1 s2 => IfS ot join (subst_l xs e) (subst_stmt xs s1) (subst_stmt xs s2)
   | Switch it e m' bs def => Switch it (subst_l xs e) m' (subst_stmt xs <$> bs) (subst_stmt xs def)
   | Assign o ot e1 e2 s => Assign o ot (subst_l xs e1) (subst_l xs e2) (subst_stmt xs s)
   | Free ly e s => Free ly (subst_l xs e) (subst_stmt xs s)
@@ -501,9 +502,9 @@ Inductive stmt_step : stmt → runtime_function → state → list Empty_set →
     v2 `has_layout_val` (ot_layout ot) →
     heap_at l (ot_layout ot) v' start_st σ.(st_heap).(hs_heap) →
     stmt_step (Assign o ot (Val v1) (Val v2) s) rf σ [] (to_rtstmt rf end_stmt) (heap_fmap (heap_upd l end_val end_st) σ) []
-| IfSS ot v s1 s2 rf σ b:
+| IfSS ot join v s1 s2 rf σ b:
     cast_to_bool ot v σ.(st_heap) = Some b →
-    stmt_step (IfS ot (Val v) s1 s2) rf σ [] (to_rtstmt rf ((if b then s1 else s2))) σ []
+    stmt_step (IfS ot join (Val v) s1 s2) rf σ [] (to_rtstmt rf ((if b then s1 else s2))) σ []
 | SwitchS rf σ v n m bs s def it :
     val_to_Z v it = Some n →
     (∀ i : nat, m !! n = Some i → is_Some (bs !! i)) →
@@ -622,7 +623,7 @@ Inductive stmt_ectx :=
 | AssignLCtx (o : order) (ot : op_type) (v2 : val) (s : stmt)
 | ReturnCtx
 | FreeCtx (ly : layout) (s : stmt)
-| IfSCtx (ot : op_type) (s1 s2 : stmt)
+| IfSCtx (ot : op_type) (join : option label) (s1 s2 : stmt)
 | SwitchCtx (it : int_type) (m: gmap Z nat) (bs : list stmt) (def : stmt)
 | ExprSCtx (s : stmt)
 .
@@ -633,7 +634,7 @@ Definition stmt_fill_item (Ki : stmt_ectx) (e : runtime_expr) : rtstmt :=
   | AssignLCtx o ot v2 s => RTAssign o ot e (Val v2) s
   | ReturnCtx => RTReturn e
   | FreeCtx ly s => RTFree ly e s
-  | IfSCtx ot s1 s2 => RTIfS ot e s1 s2
+  | IfSCtx ot join s1 s2 => RTIfS ot join e s1 s2
   | SwitchCtx it m bs def => RTSwitch it e m bs def
   | ExprSCtx s => RTExprS e s
   end.
